**Mathematical Statement:** The sum of the first \$n\$ positive integers is given by the formula:

$$ \sum_{i=1}^{n} i = \frac{n(n+1)}{2} $$

> ðŸ’¡ **Exemplo NumÃ©rico:** Let's calculate the sum of the first 5 positive integers using the formula. Here, \$n\$ = 5. So, the sum should be (5 * (5+1)) / 2 = (5 * 6) / 2 = 30 / 2 = 15. Let's verify this by directly adding the numbers: 1 + 2 + 3 + 4 + 5 = 15. The formula works!

**Proof:**

We will prove the statement using mathematical induction.

I. **Base Case:** For \$n\$ = 1, the sum is simply 1. The formula gives us (1(1+1))/2 = 1. Thus, the formula holds for \$n\$ = 1.

> ðŸ’¡ **Exemplo NumÃ©rico:** For the base case \$n\$ = 1, the formula correctly predicts the sum is 1. This serves as the foundation for our inductive proof.

II. **Inductive Hypothesis:** Assume that the formula holds for some integer \$k\$ â‰¥ 1. That is, assume:

$$ \sum_{i=1}^{k} i = \frac{k(k+1)}{2} $$

> ðŸ’¡ **Exemplo NumÃ©rico:** Suppose \$k\$ = 4. Our inductive hypothesis is that 1 + 2 + 3 + 4 = (4 * (4+1)) / 2 = (4 * 5) / 2 = 10. This assumption will be used in the next step to prove the formula for \$k\$ + 1.

III. **Inductive Step:** We need to show that the formula also holds for \$n\$ = \$k\$ + 1. That is, we need to show:

$$ \sum_{i=1}^{k+1} i = \frac{(k+1)(k+2)}{2} $$

IV. Starting with the left-hand side of the equation for \$n\$ = \$k\$ + 1, we have:

$$ \sum_{i=1}^{k+1} i = \sum_{i=1}^{k} i + (k+1) $$

> ðŸ’¡ **Exemplo NumÃ©rico:** If \$k\$ = 4, then \$k\$ + 1 = 5. So, the sum from 1 to 5 is the same as the sum from 1 to 4, plus 5. This step breaks down the problem into a part we assume to know (sum from 1 to \$k\$) and a single additional term.

V. Using the inductive hypothesis, we can substitute the sum from 1 to \$k\$:

$$ \sum_{i=1}^{k+1} i = \frac{k(k+1)}{2} + (k+1) $$

> ðŸ’¡ **Exemplo NumÃ©rico:** Using our \$k\$ = 4 example, this step substitutes the sum from 1 to 4 with the formula's result: 1 + 2 + 3 + 4 + 5 = (4 * 5) / 2 + 5.

VI. Now, let's simplify the expression:

$$ \sum_{i=1}^{k+1} i = \frac{k(k+1) + 2(k+1)}{2} = \frac{(k+1)(k+2)}{2} $$

> ðŸ’¡ **Exemplo NumÃ©rico:** Continuing with \$k\$ = 4: (4 * 5) / 2 + 5 = 10 + 5 = 15. Now, let's simplify the right-hand side according to the inductive step: ((4+1) * (4+2)) / 2 = (5 * 6) / 2 = 30 / 2 = 15. Both sides are equal, which supports the inductive step.

VII. This is exactly the right-hand side of the equation we wanted to prove. Therefore, the formula holds for \$n\$ = \$k\$ + 1.

VIII. **Conclusion:** By the principle of mathematical induction, the formula

$$ \sum_{i=1}^{n} i = \frac{n(n+1)}{2} $$

holds for all positive integers \$n\$. â– 

> ðŸ’¡ **Exemplo NumÃ©rico:** We have shown, using induction, that the formula holds for the base case (n=1) and that if it holds for \$k\$, it also holds for \$k\$+1. Therefore, it holds for all positive integers. To further test, let's use \$n\$=10: (10 * 11) / 2 = 55. Directly summing confirms this: 1+2+3+4+5+6+7+8+9+10 = 55.

```python
import numpy as np
import matplotlib.pyplot as plt

# Demonstrate the formula for different values of n
n_values = np.arange(1, 11)
sums_formula = (n_values * (n_values + 1)) / 2
sums_direct = [np.sum(np.arange(1, n+1)) for n in n_values]

plt.figure(figsize=(10, 6))
plt.plot(n_values, sums_formula, marker='o', linestyle='-', color='blue', label='Formula: n(n+1)/2')
plt.plot(n_values, sums_direct, marker='x', linestyle='--', color='red', label='Direct Sum: 1 + 2 + ... + n')
plt.title('Sum of First n Positive Integers')
plt.xlabel('n')
plt.ylabel('Sum')
plt.grid(True)
plt.legend()
plt.show()
```

The Python code above generates a plot to visually confirm the formula for different values of \$n\$. It calculates the sum using both the formula and direct summation and plots the results. The plot demonstrates that the formula and direct summation yield the same results.
<!-- END -->